src3.0/Transforms/palloca_props.v
@@ -1754,6 +1754,257 @@ Proof.
   intros. simpl in H. unfold wf_use_at_head. auto.
 Qed.
 
+Lemma WF_PhiInfo_spec6': forall (pinfo : PhiInfo) (ps1 : phinodes) (l1 : l)
+  (cs1 : cmds) (tmn1 : terminator) (H : WF_PhiInfo pinfo)
+  (HBinF : blockInFdefB (block_intro l1 ps1 cs1 tmn1) (PI_f pinfo) = true)
+  (H0 : uniqFdef (PI_f pinfo)),
+  ~ In (PI_id pinfo) (getPhiNodesIDs ps1).
+Proof.
+  intros.
+  apply blockInFdefB_lookupBlockViaLabelFromFdef in HBinF; auto.
+  eapply WF_PhiInfo_spec6; eauto.
+Qed.
+
+Lemma WF_PhiInfo_spec6'': forall (pinfo : PhiInfo) (ps1 : phinodes) (l1 : l)
+  (cs1 : cmds) (tmn1 : terminator) (H : WF_PhiInfo pinfo) F
+  (HBinF : blockInFdefB (block_intro l1 ps1 cs1 tmn1) F = true)
+  (H0 : uniqFdef F),
+  PI_f pinfo <> F \/ ~ In (PI_id pinfo) (getPhiNodesIDs ps1).
+Proof.
+  intros.
+  destruct (fdef_dec (PI_f pinfo) F); subst; auto.
+  right.
+  eapply WF_PhiInfo_spec6'; eauto.
+Qed.
+
+Ltac WF_PhiInfo_spec6_tac :=
+try solve [eapply WF_PhiInfo_spec6; eauto | 
+           eapply WF_PhiInfo_spec6'; eauto | 
+           eapply WF_PhiInfo_spec6''; eauto].
+
+Lemma switchToNewBasicBlock_doesnt_change_pid: forall pinfo l'0 ps'0 cs' tmn'0 B 
+  gl2 lc2 lc'0 td (H : WF_PhiInfo pinfo)
+  (H0 : uniqFdef (PI_f pinfo)),
+  blockInFdefB (block_intro l'0 ps'0 cs' tmn'0) (PI_f pinfo) = true ->
+  Opsem.switchToNewBasicBlock td
+         (block_intro l'0 ps'0 cs' tmn'0) B gl2 lc2 = 
+       ret lc'0 ->
+  lookupAL (GVsT DGVs) lc2 (PI_id pinfo) =
+    lookupAL (GVsT DGVs) lc'0 (PI_id pinfo).
+Proof.
+  unfold Opsem.switchToNewBasicBlock.
+  intros.
+  inv_mbind.
+  erewrite <- OpsemProps.updateValuesForNewBlock_spec7'; eauto.
+  eapply OpsemProps.getIncomingValuesForBlockFromPHINodes_spec8; eauto.
+  simpl.
+  WF_PhiInfo_spec6_tac.
+Qed.
+
+Lemma WF_PhiInfo_spec20: forall pinfo (Hwfpi: WF_PhiInfo pinfo)
+  (Huniq: uniqFdef (PI_f pinfo)),
+  lookupTypViaIDFromFdef (PI_f pinfo) (PI_id pinfo) = 
+    Some (typ_pointer (PI_typ pinfo)).
+Proof.
+  intros.
+  simpl_WF_PhiInfo.
+  destruct Hwfpi as [J1 J2].
+  symmetry in HeqR.
+  apply entryBlockInFdef in HeqR.
+  eapply uniqF__lookupTypViaIDFromFdef; eauto; simpl; auto.
+Qed.
+
+Lemma WF_PhiInfo_spec14: forall pinfo l1 ps1 cs11 t v align0 cs tmn2
+  (Hwfpi: WF_PhiInfo pinfo) (Huniq: uniqFdef (PI_f pinfo))
+  (HBinF: blockInFdefB (block_intro l1 ps1
+                 (cs11 ++ insn_alloca (PI_id pinfo) t v align0 :: cs) tmn2)
+               (PI_f pinfo) = true),
+  getEntryBlock (PI_f pinfo) =
+    ret block_intro l1 ps1
+         (cs11 ++ insn_alloca (PI_id pinfo) t v align0 :: cs) tmn2.
+Proof.
+  intros.
+  destruct Hwfpi as [Hwfpi _].
+  unfold promotable_alloca in Hwfpi.
+  inv_mbind. symmetry_ctx.
+  destruct b as [l0 ps0 cs0 tmn0].
+  f_equal.
+  eapply block_eq1 with (id0:=PI_id pinfo); eauto.
+    apply entryBlockInFdef in HeqR.
+    eapply inGetBlockIDs__lookupBlockViaIDFromFdef; eauto.
+    destruct Hwfpi as [J _].
+    eapply getCmdID_in_getBlocksIDs; eauto. 
+      simpl; auto.
+
+    eapply getCmdID_in_getBlocksIDs; eauto using in_middle.
+      simpl; auto.
+Qed.
+
+Lemma WF_PhiInfo_spec16: forall pinfo S los nts Ps,
+  WF_PhiInfo pinfo ->
+  wf_fdef S (module_intro los nts Ps) (PI_f pinfo) ->
+  exists sz, exists al,
+    getTypeSizeInBits_and_Alignment (los,nts) true (PI_typ pinfo) = 
+      Some (sz, al) /\ 
+    (sz > 0)%nat /\ (al > 0)%nat.
+Proof.
+  intros.
+  simpl_WF_PhiInfo.
+  destruct H as [J1 J2].
+  symmetry in HeqR.
+  apply entryBlockInFdef in HeqR.
+  eapply wf_fdef__wf_cmd in HeqR; eauto.
+  inv HeqR.
+  eapply wf_typ__getTypeSizeInBits_and_Alignment in H12; eauto.
+Qed.
+
+Ltac WF_PhiInfo_spec10_tac :=
+repeat match goal with
+| HBinF2 : blockInFdefB ?B' (PI_f ?pinfo) = true,
+  Heq3' : exists l1 : l,
+            exists ps1 : phinodes,
+              exists cs11 : list cmd,
+                ?B' =
+                block_intro l1 ps1
+                  (cs11 ++ _ :: ?cs') ?tmn3 |- _ =>
+  destruct Heq3' as [l2 [ps2 [cs21 Heq3']]]; subst;
+  eapply WF_PhiInfo_spec10 in HBinF2; eauto 2 using wf_system__uniqFdef
+| HBinF2 : blockInFdefB ?B' ?F = true,
+  Heq3' : exists l1 : l,
+            exists ps1 : phinodes,
+              exists cs11 : list cmd,
+                ?B' =
+                block_intro l1 ps1
+                  (cs11 ++ _ :: ?cs') ?tmn3 |- 
+  ?A <> ?F \/ _ => destruct (fdef_dec A F); subst; auto; right
+end.
+
+Ltac solve_non_pid_updateAddAL :=
+match goal with
+| HBinF2 : blockInFdefB ?B' ?F' = true,
+  Heq3' : exists l1 : l,
+            exists ps1 : phinodes,
+              exists cs11 : list cmd,
+                ?B' =
+                block_intro l1 ps1
+                  (cs11 ++ _ :: ?cs') ?tmn3 |-
+  PI_f _ = ?F' ->
+  lookupAL _ ?lc ?id1 =
+  lookupAL _ (updateAddAL _ ?lc _ _ ) ?id1=>
+  intro; subst;
+  rewrite <- lookupAL_updateAddAL_neq; auto;
+  WF_PhiInfo_spec10_tac
+end.
+
+Lemma WF_PhiInfo_spec19: forall B pinfo (Huniq: uniqFdef (PI_f pinfo))
+  (Hwfpi: WF_PhiInfo pinfo)
+  (HBinF: blockInFdefB B (PI_f pinfo))
+  (Hin: In (PI_id pinfo) (getBlockLocs B)),
+  getEntryBlock (PI_f pinfo) = Some B.
+Proof.
+  intros.
+  simpl_WF_PhiInfo.
+  f_equal.
+  eapply block_eq2; eauto 2.
+    symmetry_ctx.
+    solve_blockInFdefB.
+
+    destruct Hwfpi. simpl in *.
+    apply getCmdLoc_in_getCmdsLocs in H. simpl in H.
+    xsolve_in_list.
+Qed.
+
+Lemma WF_PhiInfo_spec1': forall pinfo l1 ps1 cs11 c1 cs1 tmn2,
+  WF_PhiInfo pinfo ->
+  uniqFdef (PI_f pinfo) ->
+  blockInFdefB (block_intro l1 ps1 (cs11 ++ c1 :: cs1) tmn2) (PI_f pinfo) 
+    = true ->
+  PI_id pinfo = getCmdLoc c1 ->
+  c1 = insn_alloca (PI_id pinfo) (PI_typ pinfo) (PI_num pinfo)
+         (PI_align pinfo).
+Proof.
+  intros.
+  assert (In (PI_id pinfo) 
+    (getBlockLocs (block_intro l1 ps1 (cs11 ++ c1 :: cs1) tmn2))) as Hin.
+    simpl. rewrite H2. xsolve_in_list.
+  eapply WF_PhiInfo_spec19 in Hin; eauto.
+  simpl_WF_PhiInfo. inv Hin.
+  destruct H.
+  eapply NoDup_getCmdsLocs_prop; eauto using in_middle.
+    solve_NoDup.
+Qed.
+
+Definition args_dont_use_pid pinfo F (la:list (typ * attributes * id)) :=
+  PI_f pinfo <> F \/ (forall t a i0, In (t,a,i0) la -> PI_id pinfo <> i0).
+
+Lemma WF_PhiInfo__args_dont_use_pid: forall pinfo F la0
+  (Huniq: uniqFdef F) (Hneq: la0 = getArgsOfFdef F) (Hwfpi: WF_PhiInfo pinfo),
+  args_dont_use_pid pinfo F la0.
+Proof.
+  intros.
+  unfold args_dont_use_pid.
+  destruct (fdef_dec (PI_f pinfo) F); subst; auto.
+  right.
+  apply WF_PhiInfo_spec1 in Hwfpi; auto.
+  destruct (PI_f pinfo) as [[]]. simpl. intros.
+  eapply IngetArgsIDs__lookupCmdViaIDFromFdef with (id0:=i0) in Huniq; eauto.
+    congruence.
+    eapply In_getArgsIDs_spec; eauto.
+Qed.
+
+Lemma WF_PhiInfo__pid_isnt_in_init: forall pinfo (Hwfpi: WF_PhiInfo pinfo)
+  (Huniq: uniqFdef (PI_f pinfo)) lc VarArgs TD
+  (Hinit: @Opsem.initLocals DGVs TD (getArgsOfFdef (PI_f pinfo)) VarArgs = ret lc),
+  lookupAL _ lc (PI_id pinfo) = None.
+Proof.
+  intros.
+  remember (lookupAL (GVsT DGVs) lc (PI_id pinfo)) as R.
+  destruct R; auto.
+  eapply OpsemProps.In_initLocals__In_getArgsIDs with (id1:=PI_id pinfo) in Hinit; 
+    eauto.
+  apply WF_PhiInfo_spec1 in Hwfpi; auto.
+  destruct (PI_f pinfo) as [[]].
+  eapply IngetArgsIDs__lookupCmdViaIDFromFdef in Huniq; eauto.
+  congruence.
+Qed.
+
+Lemma WF_PhiInfo_spec21: forall pinfo (Hwfpi : WF_PhiInfo pinfo)
+  (los : layouts) (nts : namedts) (Ps : products) S 
+  (HUniq: uniqFdef (PI_f pinfo))
+  (HwfF : wf_fdef S (module_intro los nts Ps) (PI_f pinfo)),
+  wf_typ S (los, nts) (PI_typ pinfo).
+Proof.
+  intros.
+  apply WF_PhiInfo_spec1 in Hwfpi; auto.
+  apply lookupInsnViaIDFromFdef__insnInFdefBlockB in Hwfpi.
+  destruct Hwfpi as [b1 Hwfpi].
+  apply destruct_insnInFdefBlockB in Hwfpi.
+  destruct Hwfpi as [J1 J2]. 
+  destruct b1. simpl in *.
+  apply InCmdsB_in in J1.
+  eapply wf_fdef__wf_cmd in J2; eauto.
+  inv J2. auto.
+Qed.
+
+Lemma WF_PhiInfo_spec22: forall pinfo (Hwfpi : WF_PhiInfo pinfo)
+  (los : layouts) (nts : namedts) (Ps : products)  
+  (HUniq: uniqFdef (PI_f pinfo)),
+  exists l0, exists ps0, exists cs1, exists cs2, exists tmn0,
+    getEntryBlock (PI_f pinfo) = 
+      Some (block_intro l0 ps0 
+        (cs1 ++ insn_alloca (PI_id pinfo) (PI_typ pinfo) 
+           (PI_num pinfo) (PI_align pinfo):: cs2) tmn0).
+Proof.
+  intros.
+  simpl_WF_PhiInfo.
+  exists l5. exists phinodes5.
+  destruct Hwfpi as [J1 J2].
+  apply in_split in J1.
+  destruct J1 as [cs1 [cs2 J1]]; subst.
+  exists cs1. exists cs2. exists terminator5.
+  auto.
+Qed.
+
 (***************************************************************************)
 (*           pid is not defined until the allocation in entry              *)
 
@@ -2256,32 +2507,6 @@ Proof.
   eapply preservation_star; eauto.
 Qed.  
 
-Lemma WF_PhiInfo_spec14: forall pinfo l1 ps1 cs11 t v align0 cs tmn2
-  (Hwfpi: WF_PhiInfo pinfo) (Huniq: uniqFdef (PI_f pinfo))
-  (HBinF: blockInFdefB (block_intro l1 ps1
-                 (cs11 ++ insn_alloca (PI_id pinfo) t v align0 :: cs) tmn2)
-               (PI_f pinfo) = true),
-  getEntryBlock (PI_f pinfo) =
-    ret block_intro l1 ps1
-         (cs11 ++ insn_alloca (PI_id pinfo) t v align0 :: cs) tmn2.
-Proof.
-  intros.
-  destruct Hwfpi as [Hwfpi _].
-  unfold promotable_alloca in Hwfpi.
-  inv_mbind. symmetry_ctx.
-  destruct b as [l0 ps0 cs0 tmn0].
-  f_equal.
-  eapply block_eq1 with (id0:=PI_id pinfo); eauto.
-    apply entryBlockInFdef in HeqR.
-    eapply inGetBlockIDs__lookupBlockViaIDFromFdef; eauto.
-    destruct Hwfpi as [J _].
-    eapply getCmdID_in_getBlocksIDs; eauto. 
-      simpl; auto.
-
-    eapply getCmdID_in_getBlocksIDs; eauto using in_middle.
-      simpl; auto.
-Qed.
-
 Lemma WF_PhiInfo_spec15: forall (pinfo : PhiInfo) (tmn2 : terminator)
   (lc2 : Opsem.GVsMap) (als2 : list mblock) (Hwfpi : WF_PhiInfo pinfo)
   (B : block) (t : typ) (v : value)
@@ -2328,24 +2553,6 @@ Proof.
       eapply uniqFdef_cmds_split_middle; eauto.
     destruct G; subst.
     exists cs1. exists nil. auto.
-Qed.
-
-Lemma WF_PhiInfo_spec16: forall pinfo S los nts Ps,
-  WF_PhiInfo pinfo ->
-  wf_fdef S (module_intro los nts Ps) (PI_f pinfo) ->
-  exists sz, exists al,
-    getTypeSizeInBits_and_Alignment (los,nts) true (PI_typ pinfo) = 
-      Some (sz, al) /\ 
-    (sz > 0)%nat /\ (al > 0)%nat.
-Proof.
-  intros.
-  simpl_WF_PhiInfo.
-  destruct H as [J1 J2].
-  symmetry in HeqR.
-  apply entryBlockInFdef in HeqR.
-  eapply wf_fdef__wf_cmd in HeqR; eauto.
-  inv HeqR.
-  eapply wf_typ__getTypeSizeInBits_and_Alignment in H12; eauto.
 Qed.
 
 Lemma s_genInitState__palloca: forall S main VarArgs cfg IS pinfo
@@ -2429,12 +2636,6 @@ end.
       admit. (* should find_init_stld check typ and align matches? *)
 Qed.
 
-Ltac destruct_dec :=
-match goal with
-| |- context [id_dec ?b ?a] =>
-  destruct (id_dec b a); subst; try congruence; auto
-end.
-
 Ltac find_next_stld_spec_tac :=
 match goal with
 | H: Some _ = _,
@@ -2512,4 +2713,125 @@ Proof.
       split; auto.
         admit. (* should find_next_stld check typ and align matches? *)
 Qed.
+
+(*************************************)
+(* Aux invariants of wf ECs *)
+
+(* go to infra *)
+Definition wfEC_inv s m (EC: @Opsem.ExecutionContext DGVs) : Prop :=
+uniqFdef (Opsem.CurFunction EC) /\ 
+blockInFdefB (Opsem.CurBB EC) (Opsem.CurFunction EC) = true /\
+match Opsem.CurCmds EC with
+| nil => wf_insn s m (Opsem.CurFunction EC) (Opsem.CurBB EC) 
+           (insn_terminator (Opsem.Terminator EC))
+| c::_ => wf_insn s m (Opsem.CurFunction EC) (Opsem.CurBB EC) 
+           (insn_cmd c)
+end /\
+exists l0, exists ps0, exists cs0,
+  Opsem.CurBB EC = block_intro l0 ps0 (cs0 ++ Opsem.CurCmds EC)
+    (Opsem.Terminator EC).
+
+(* go to infra *)
+Definition wfECs_inv s m (ECs: list (@Opsem.ExecutionContext DGVs)) : Prop :=
+List.Forall (wfEC_inv s m) ECs.
+
+(* go to infra *)
+Lemma wf_EC__wfEC_inv: forall S los nts Ps EC
+  (HwfS : wf_system S) 
+  (HMinS : moduleInSystemB (module_intro los nts Ps) S = true)
+  (Hwfec : OpsemPP.wf_ExecutionContext (los, nts) Ps EC),
+  wfEC_inv S (module_intro los nts Ps) EC.
+Proof.
+  destruct EC; simpl.
+  intros.
+  destruct Hwfec as [J1 [J2 [J3 [J4 [J5 J6]]]]].
+  unfold wfEC_inv. simpl.
+  split; eauto 2 using wf_system__uniqFdef.
+  split; auto.
+  split; auto.
+    destruct J6 as [l1 [ps1 [cs1 J6]]]; subst.
+    destruct CurCmds.
+      eapply wf_system__wf_tmn in J2; eauto.
+      eapply wf_system__wf_cmd in J2; eauto using in_middle.
+Qed.
+
+(* go to infra *)
+Lemma wf_ECStack__wfECs_inv: forall S los nts Ps ECs
+  (HwfS : wf_system S) 
+  (HMinS : moduleInSystemB (module_intro los nts Ps) S = true)
+  (Hwf : OpsemPP.wf_ECStack (los, nts) Ps ECs),
+  wfECs_inv S (module_intro los nts Ps) ECs.
+Proof.
+  unfold wfECs_inv.
+  induction ECs as [|]; simpl; intros; auto.
+    destruct Hwf as [J1 [J2 J3]].
+    constructor; eauto using wf_EC__wfEC_inv.
+Qed.
+
+(* go to infra *)
+Lemma wf_State__wfECs_inv: forall cfg St (Hwfc: OpsemPP.wf_Config cfg) 
+  (Hwfst: OpsemPP.wf_State cfg St), 
+  wfECs_inv (OpsemAux.CurSystem cfg) 
+    (module_intro (fst (OpsemAux.CurTargetData cfg))
+                  (snd (OpsemAux.CurTargetData cfg))
+                  (OpsemAux.CurProducts cfg) )
+    (Opsem.ECS St).
+Proof.
+  intros.
+  destruct cfg as [? [? ?] ? ?].
+  destruct St.
+  destruct Hwfc as [? [? [? ?]]].
+  destruct Hwfst. simpl.
+  eapply wf_ECStack__wfECs_inv; eauto.
+Qed.
+
+(* go to infra *)
+Definition uniqEC (EC: @Opsem.ExecutionContext DGVs) : Prop :=
+uniqFdef (Opsem.CurFunction EC) /\ 
+blockInFdefB (Opsem.CurBB EC) (Opsem.CurFunction EC) = true /\
+exists l0, exists ps0, exists cs0,
+  Opsem.CurBB EC = block_intro l0 ps0 (cs0 ++ Opsem.CurCmds EC)
+    (Opsem.Terminator EC).
+
+(* go to infra *)
+Definition uniqECs (ECs: list (@Opsem.ExecutionContext DGVs)) : Prop :=
+List.Forall uniqEC ECs.
+
+Lemma wfEC_inv__uniqEC: forall s m EC (Hwf: wfEC_inv s m EC), uniqEC EC.
+Proof.
+  intros.
+  destruct Hwf as [J1 [J3 [_ J2]]]. split; auto.
+Qed.
+
+Lemma wfECs_inv__uniqECs: forall s m ECs (Hwf: wfECs_inv s m ECs), uniqECs ECs.
+Proof.
+  unfold wfECs_inv, uniqECs.
+  intros.
+  induction Hwf; auto.
+    constructor; auto.
+      apply wfEC_inv__uniqEC in H; auto.
+Qed.
+
+(* go to infra *)
+Lemma wf_State__uniqECs: forall cfg St (Hwfc: OpsemPP.wf_Config cfg) 
+  (Hwfst: OpsemPP.wf_State cfg St), uniqECs (Opsem.ECS St).
+Proof.
+  intros.
+  destruct cfg as [? [? ?] ? ?].
+  destruct St.
+  destruct Hwfc as [? [? [? ?]]].
+  destruct Hwfst. simpl.
+  eapply wf_ECStack__wfECs_inv in H4; eauto.
+  eapply wfECs_inv__uniqECs; eauto.
+Qed.
+
+Ltac find_uniqEC :=
+repeat match goal with
+| H: uniqECs (Opsem.ECS {|Opsem.ECS := _; Opsem.Mem := _ |}) |- uniqEC _ => 
+  simpl in H
+| H: uniqECs (?EC::_) |- uniqEC ?EC => inv H; auto
+| H: uniqECs (_::?EC::_) |- uniqEC ?EC => inv H; auto
+| H: Forall uniqEC (?EC::_) |- uniqEC ?EC => inv H; auto
+| H: Forall uniqEC (_::?EC::_) |- uniqEC ?EC => inv H; auto
+end.
 
